eclib/JWord_array.ec
@@ -252,21 +252,20 @@ abstract theory WArray.
 
   (* ------------------------------------------------- *)
 
-  clone import PolyArray as ArrayW8.
+  clone PolyArray as ArrayW8.
 
-  op of_array8 (a: W8.t ArrayW8.t) = init8 (fun i -> a.[i]).
+  op of_array8 (a: W8.t ArrayW8.t) = init8 (ArrayW8."_.[_]" a).
 
-  op to_array8 (a: t) = ArrayW8.init (fun i -> get8 a i).
+  op to_array8 (a:t) = ArrayW8.init (fun i => get8 a i).
 
-
+  (*
 op (a: ArrayN' Wws): WArrayN.initWS (fun i -> a.[i])
 op (a: WArrayN'): ArrayN.init (fun i -> getWS a i)
-  
-
+    *)
 end WArray.
 
 (* Array of words, where the word size is any number of bytes *)
-abstract theory ArrayWords
+abstract theory ArrayWords.
     (* size of a word in bytes *)
     op sizeW: int.
     axiom gt0_sizeW: 0 < sizeW.
@@ -275,36 +274,41 @@ abstract theory ArrayWords
     op sizeA: int.
     axiom gt0_sizeA: 0 < sizeA.
 
-    clone BitWord as Word with
+    clone WT as Word with
         op size <- 8 * sizeW
-        proof gt0_size by done.
+        proof gt0_size by rewrite pmulr_rgt0 // gt0_sizeW.
 
-    clone PolyArray as ArrayN with
-        size <= sizeA
-        proof ge0_size by done.
+    clone import PolyArray as ArrayN with
+        op size <- sizeA
+        proof ge0_size by rewrite ltzW gt0_sizeA.
 
     (* Equivalent array of bytes *)
-    clone WArray as WArrayN with
-        size <= sizeW * sizeA
-        proof ge0_size by done.
+    clone import WArray as WArrayN with
+        op size <- sizeW * sizeA
+        proof ge0_size by rewrite pmulr_rge0 1:gt0_sizeW ltzW gt0_sizeA.
 
     (* Conversion between WArrayN.t and Word.t ArrayN.t *)
+        (* Cannot be done because requires WT as word and not BitWord
+        (<<, ... operators)
+    Probably we need some WT.
+          *)
     clone W_WS as Wu8 with
-        op sizeS <- W8.size, op sizeB <- Word.size, op r <- sizeW,
-        theory WS <- W8, theory WB <- Word
-        proof gt0_r by done, sizeBrS by done.
+        op sizeS <= W8.size, op sizeB <= W8.size*sizeW, op r <= sizeW,
+        theory WS <= W8, theory WB <= Word
+        proof gt0_r by apply gt0_sizeW, sizeBrS by rewrite mulzC.
 
     (* direct means offset in bytes, not in words *)
+        (* TODO: we don't have Wu8 so we can't do this. Check what is done by current extraction ? *)
     op wa_get_direct (t: WArrayN.t) (i: int): Word.t =
-        Wu8.pack'R_t (Wu8.Pack.init (fun j => t.[i+j])).
+        Wu8.pack'R_t (Wu8.Pack.init (fun j => WArrayN.get8 t (i+j))).
     abbrev wa_get (t: WArrayN.t) (i: int): Word.t = wa_get_direct t (sizeW*i).
     op wa_set_direct (t: WArrayN.t) (i: int) (w: Word.t) =
-        WArrayN.init (fun k => if i <= k < i + sizeW then w \bits8 (k-i) else t.[k]).
+        WArrayN.init (fun k => if i <= k < i + sizeW then Wu8.\bits'S w (k-i) else t.[k]).
 
     op of_word_array (a: Word.t ArrayN.t) =
-        WArrayN.init (fun i => a.[i %/ sizeW] \bits8 (i%%sizeW)).
+        WArrayN.init (fun i => Wu8.\bits'S a.[i %/ sizeW] (i%%sizeW)).
     op to_word_array (a: WArrayN.t) =
-        ArrayN.init (fun i -> wa_get a i).
+        ArrayN.init (fun i => wa_get a i).
 
     op get_direct (a: Word.t ArrayN.t) = wa_get_direct (of_word_array a).
     op set_direct (a: Word.t ArrayN.t) (i: int) (w: Word.t) =
@@ -321,19 +325,19 @@ theory SubArray.
     axiom gt0_sizeB: 0 < sizeB.
 
     (* Sub-array *)
-    clone PolyArray as ArrayS with
-        size <= sizeS
-        proof ge0_size by done.
+    clone import PolyArray as ArrayS with
+        op size <- sizeS
+        proof ge0_size by rewrite ltzW gt0_sizeS.
 
     (* Base array *)
-    clone PolyArray as ArrayB with
-        size <= sizeB
-        proof ge0_size by done.
+    clone import PolyArray as ArrayB with
+        op size <- sizeB
+        proof ge0_size by rewrite ltzW gt0_sizeB.
 
-  op get_sub (a: 'a ArrayB.t) (i: int) = ArrayS.init (fun j -> a.[i + j]).
+  op get_sub (a: 'a ArrayB.t) (i: int) = ArrayS.init (fun j => a.[i + j]).
 
   op set_sub (a: 'a ArrayB.t) (i: int) (b: 'a ArrayS.t) =
-    ArrayB.init (fun j -> if i <= j < i + sizeS then b.[j - i] else a.[j]).
+    ArrayB.init (fun j => if i <= j < i + sizeS then b.[j - i] else a.[j]).
 end SubArray.
 
 theory SubArrayDirect.
@@ -346,82 +350,32 @@ theory SubArrayDirect.
     op sizeB: int.
     axiom gt0_sizeB: 0 < sizeB.
 
-    clone BitWord as Word with
+    clone WT as Word with
         op size <- 8 * sizeW
-        proof gt0_size by done.
+        proof gt0_size by rewrite pmulr_rgt0 1:// gt0_sizeW.
 
     clone ArrayWords as ArrayWordsS with
         op sizeW <- sizeW, op sizeA <- sizeS, theory Word <- Word
-        proof gt0_sizeW by done, gt0_sizeA by done.
+        proof gt0_sizeW by apply gt0_sizeW, gt0_sizeA by apply gt0_sizeS.
 
     clone ArrayWords as ArrayWordsB with
         op sizeW <- sizeW, op sizeA <- sizeB, theory Word <- Word
-        proof gt0_sizeW by done, gt0_sizeA by done.
+        proof gt0_sizeW by apply gt0_sizeW, gt0_sizeA by apply gt0_sizeB.
 
     op get_sub_direct (a: Word.t ArrayWordsB.ArrayN.t) (i: int) =
-        ArrayWordsS.ArrayN.init (fun j -> ArrayWordsB.get_direct a (i + j)).
+        ArrayWordsS.ArrayN.init (fun j => ArrayWordsB.get_direct a (i + j)).
 
-    op set_sub_direct (a: W16.t ArrayB.t) (i: int) (b: W16.t ArrayS.t) =
-        let aw = ArrayWordsB.of_word_array a in
-        let bw = ArrayWordsS.of_word_array b in
-        (* FIXME: change init8 and get8 to init and _.[_] *)
+    op set_sub_direct (a: Word.t ArrayWordsB.ArrayN.t) (i: int) (b: Word.t ArrayWordsS.ArrayN.t) =
+        (* FIXME: change init8 and get8 to init and _.[_] (breaks compatibility by rewrite) *)
         ArrayWordsB.to_word_array (
-            ArrayWordsB.WArrayN.init8 (fun j ->
-            if i <= j < i * sizeW * sizeS then get8 bw (j - i) else get8 aw j
+            ArrayWordsB.WArrayN.init8 (fun j =>
+            if i <= j < i * sizeW * sizeS then
+                ArrayWordsS.WArrayN.get8 (ArrayWordsS.of_word_array b) (j - i)
+            else
+                ArrayWordsB.WArrayN.get8 (ArrayWordsB.of_word_array a) j
             )
         ).
 end SubArrayDirect.
-
-(*
-theory ArrayWords16.
-  op size: int.
-  clone PolyArray as ArrayN with size <= size.
-  clone WArray as WArrayN with size <= 2 * size.
-  (* FIXME: prove axioms of cloned theories. *)
-
-  op of_w16_array (a: W16.t ArrayN.t) = WArrayN.init16 (fun i -> a.[i]).
-  op to_w16_array (a: WArrayN.t) = ArrayN.init (fun i -> get16 a i).
-
-  op get16_direct (a: W16.t ArrayN.t) = WArrayN.get16_direct (of_w16_array a).
-  op set16_direct (a: W16.t ArrayN.t) (i: int) (w: W16.t) =
-    to_w16_array (WArrayN.set16_direct (of_w16_array a) i w).
-
-end ArrayWords16.
-
-theory SubArray16Direct.
-  op sizeS: int.
-  op sizeB: int.
-
-  clone ArrayWords16 as ArrayWords16S with size <= sizeS.
-  clone ArrayWords16 as ArrayWords16B with size <= sizeB.
-
-  op get_sub_direct (a: W16.t ArrayB.t) (i: int) =
-    ArrayWords16S.ArrayN.init (fun j -> get16_direct (ArrayWords16B.of_w16_array a) (i + j)).
-
-
-  op set_sub_direct (a: W16.t ArrayB.t) (i: int) (b: W16.t ArrayS.t) =
-    let aw = ArrayWords16B.of_w16_array a in
-    let bw = ArrayWords16S.of_w16_array b in
-    (* FIXME: change init8 and get8 to init and _.[_] *)
-      ArrayWords16B.to_w16_array (
-        ArrayWords16B.WArrayN.init8 (fun j ->
-          if i <= j < i * 2 * sizeS then get8 bw (j - i) else get8 aw j
-        )
-      ).
-
-end SubArray16Direct.
-*)
-
-(* TODO: do this for pairs of Wsizes. Do this as generic theory. exemple: JWord.ec, theory W_WS and clones. *)
-
-
-(*
-from Jasmin require import JWord_array.
-require import Array8.
-
-clone export WArray as WArray8  with op size <- 8.
-clone export ArrayWords8 as ArrayWords8_8 with op size <- 8, theory ArrayN <- Array8, theory WArrayN <- WArray8.
-*)
 
 
  
